Track events in cexec
Event list itself doesn't attribute acquires/releases to a thread, but
induction over execution will tell you which program's they are by
virtue of which constructor was used. Note that the new_events added by
rstep is always empty or a singleton acq or rel, just looking at all the
constructors of rstep.

src/CSL.v
@@ -270,32 +270,35 @@ Section ConcurrentSepLogic.
       PFinished m ret1 ret2
     end.
 
-  (* TODO: track events *)
-  Inductive cexec : mem -> pstate -> pstate -> poutcomes -> Prop :=
-  | CProg1Step : forall m m' ls1 ls1' p1 p1' events p2 ls2 outs,
-      rstep (State m ls1) p1 (State m' ls1') p1' events ->
+  Inductive cexec : mem -> pstate -> pstate -> list exec_label -> poutcomes -> Prop :=
+  | CProg1Step : forall m m' ls1 ls1' p1 p1' events new_events p2 ls2 outs,
+      rstep (State m ls1) p1 (State m' ls1') p1' new_events ->
       (forall r, In r ls1' -> In r ls2 -> False) ->
-      cexec m' (PState p1' ls1') (PState p2 ls2) outs ->
-      cexec m (PState p1 ls1) (PState p2 ls2) outs
-  | CProg2Step : forall m p1 ls1 m' ls2 ls2' p2 p2' events outs,
-      rstep (State m ls2) p2 (State m' ls2') p2' events ->
+      cexec m' (PState p1' ls1') (PState p2 ls2) events outs ->
+      cexec m (PState p1 ls1) (PState p2 ls2) (new_events ++ events) outs
+  | CProg2Step : forall m p1 ls1 m' ls2 ls2' p2 p2' events new_events outs,
+      rstep (State m ls2) p2 (State m' ls2') p2' new_events ->
       (forall r, In r ls2' -> In r ls1 -> False) ->
-      cexec m' (PState p1 ls1) (PState p2' ls2') outs ->
-      cexec m (PState p1 ls1) (PState p2 ls2) outs
-  | CProg1Done : forall m m' ret1 ret2 events p2 ls2,
-      rexec (State m ls2) p2 events (Finished m' ret2) ->
-      cexec m (PState (CDone ret1) nil) (PState p2 ls2) (PFinished m' ret1 ret2)
-  | CProg2Done : forall m m' ret1 ret2 events ls1 p1,
-      rexec (State m ls1) p1 events (Finished m' ret2) ->
-      cexec m (PState p1 ls1) (PState (CDone ret2) nil) (PFinished m' ret1 ret2)
+      cexec m' (PState p1 ls1) (PState p2' ls2') events outs ->
+      cexec m (PState p1 ls1) (PState p2 ls2) (new_events ++ events) outs
+  | CProg1Done : forall m m' ret1 ret2 new_events p2 ls2,
+      rexec (State m ls2) p2 new_events (Finished m' ret2) ->
+      cexec m (PState (CDone ret1) nil) (PState p2 ls2)
+            new_events (PFinished m' ret1 ret2)
+  | CProg2Done : forall m m' ret1 ret2 new_events ls1 p1,
+      rexec (State m ls1) p1 new_events (Finished m' ret2) ->
+      cexec m (PState p1 ls1) (PState (CDone ret2) nil)
+            new_events (PFinished m' ret1 ret2)
   | CProg1Fail : forall m ls1 p1 ps2,
         (forall m' ls1' p1' events, ~rstep (State m ls1) p1 (State m' ls1') p1' events) ->
         (forall v, p1 <> CDone v) ->
-        cexec m (PState p1 ls1) ps2 PFailed
+        cexec m (PState p1 ls1) ps2
+              nil PFailed
   | CProg2Fail : forall m ps1 ls2 p2,
         (forall m' ls2' p2' events, ~rstep (State m ls2) p2 (State m' ls2') p2' events) ->
         (forall v, p2 <> CDone v) ->
-        cexec m ps1 (PState p2 ls2) PFailed.
+        cexec m ps1 (PState p2 ls2)
+              nil PFailed.
 
   Ltac inv_pstate :=
     match goal with
@@ -305,7 +308,7 @@ Section ConcurrentSepLogic.
 
   Ltac ind_cexec :=
     match goal with
-    | [ H: cexec _ ?ps1 ?ps2 ?pout |- _ ] =>
+    | [ H: cexec _ ?ps1 ?ps2 _ ?pout |- _ ] =>
       remember_nonvar ps1;
         remember_nonvar ps2;
         remember_nonvar pout;
@@ -313,8 +316,8 @@ Section ConcurrentSepLogic.
         repeat inv_pstate
     end.
 
-  Theorem locks_disjoint : forall m p1 ls1 p2 ls2 m' ret1 ret2,
-      cexec m (PState p1 ls1) (PState p2 ls2) (PFinished m' ret1 ret2) ->
+  Theorem locks_disjoint : forall m p1 ls1 p2 ls2 m' events ret1 ret2,
+      cexec m (PState p1 ls1) (PState p2 ls2) events (PFinished m' ret1 ret2) ->
       (forall r, In r ls1 -> In r ls2 -> False).
   Proof.
     Hint Resolve in_eq in_cons remove_In.
@@ -334,7 +337,7 @@ Section ConcurrentSepLogic.
     forall m d events out,
       m |= pre d * inv gamma ->
       (forall r rm, In (AcqStep r rm) events -> rinv r gamma rm) ->
-      cexec m (PState p1 nil) (PState p2 nil) out ->
+      cexec m (PState p1 nil) (PState p2 nil) events out ->
       (forall r rm, In (RelStep r rm) events -> rinv r gamma rm) /\
       (exists m' ret1 ret2, out = PFinished m' ret1 ret2 /\
                        (m' |= d ret1 ret2 * inv gamma)).
